\section{Tutorial to set up the Hubbard model}
The $SU(2)$ symmetric Hubbard model is given by
\begin{equation}
\label{eqn_hubbard_sun}
\mathcal{H}=
-t\sum\limits_{\langle i,j\rangle,\sigma} 
\left(c^{\dagger}_{i,\sigma} c^{\phantom\dagger}_{j,\sigma} + \text{H.c.}
\right)
+ \frac{U}{2}\sum\limits_{i}\left[
\sum\limits_{\sigma}
\left(  c^{\dagger}_{i\sigma} c^{\phantom\dagger}_{i\sigma}  -1/2 \right) \right]^{2}\;.
\end{equation}
To bring Eq.~(\ref{eqn_hubbard_sun}) in the general form (\ref{eqn_general_ham2}), we set
\begin{eqnarray}
N_{fl}&=&1\nonumber\\
N_{sun}&=&2\nonumber\\
T_{\bm{x}\bm{y}}&=&-t\delta_{\langle i,j\rangle}\delta_{\sigma,\sigma^{\prime}}\nonumber\\
M&=&N_{sites}\nonumber\\
U_{k}&=&-U/2\nonumber\\
V_{\bm{x}\bm{y}}^{(k)}&=&\delta_{i,j}\delta_{i,k}\delta_{\sigma,\sigma^{\prime}}\nonumber\\
\alpha_{k}&=&1/(N_{sites}N_{sun})^{2}=1/(2 N_{sites})^{2}\;.
\end{eqnarray}